src/lib/kuiper/Kuiper.ForEvery.fsti
@@ -661,6 +661,28 @@ fn forevery_map'
   ensures
     forall+ (x:b). p2 x
 
+ghost
+fn forevery_zip_2
+  (#a:Type0) {| enumerable a |}
+  (#b:Type0) {| enumerable b |}
+  (p1 p2 : a -> b -> slprop)
+  requires
+    (forall+ (x:a) (y:b). p1 x y) **
+    (forall+ (x:a) (y:b). p2 x y)
+  ensures
+    forall+ (x:a) (y:b). p1 x y ** p2 x y
+
+ghost
+fn forevery_unzip_2
+  (#a:Type0) {| enumerable a |}
+  (#b:Type0) {| enumerable b |}
+  (p1 p2 : a -> b -> slprop)
+  requires
+    forall+ (x:a) (y:b). p1 x y ** p2 x y
+  ensures
+    (forall+ (x:a) (y:b). p1 x y) **
+    (forall+ (x:a) (y:b). p2 x y)
+
 unfold
 let pad_f (#n1 : nat) (n2 : nat{n1 <= n2})
   (f : natlt n1 -> slprop)
