src/lib/poly/gemm/Kuiper.Poly.GEMM.TensorCore2D.KernelDesc.fst
@@ -1,0 +1,812 @@
+module Kuiper.Poly.GEMM.TensorCore2D.KernelDesc
+
+#lang-pulse
+
+
+#push-options "--debug SMTFail"
+// #set-options "--split_queries always"
+#set-options "--z3rlimit 40"
+
+open Kuiper
+
+open Kuiper.Matrix.Reprs
+module R = Kuiper.Matrix.Reprs
+open Kuiper.TensorCore
+
+module SZ = Kuiper.SizeT
+open Kuiper.Matrix.Reprs.Type
+open Kuiper.Math { even, odd, even_2x, odd_2x1 }
+
+open Kuiper.Array.Vectorized { has_vec_cpy, chunk }
+open Kuiper.Matrix
+
+module MS = Kuiper.Spec.GEMM
+module SZ = Kuiper.SizeT
+module B = Kuiper.Barrier
+
+open Kuiper.Matrix.Reprs
+module R = Kuiper.Matrix.Reprs
+
+open Kuiper.EMatrix
+open Kuiper.VArray {
+  varray,
+  varray_pts_to,
+  varray_pts_to_cell
+}
+open Kuiper.TensorCore
+open Kuiper.Float16
+open Kuiper.Matrix.Tiling
+
+open Kuiper.Poly.GEMM.Copy.Vec
+open Kuiper.Poly.GEMM.Tiled.Common.Vec
+
+open Pulse.Lib.Array
+open Pulse.Lib.Trade
+
+open Kuiper.Bijection
+
+ghost
+fn gpu_matrix_untile_underspec
+  (#et:Type0)
+  (#rows #cols : nat)
+  (#l : mlayout rows cols)
+  (gm : gpu_matrix et l)
+  (trows : pos { trows /? rows })
+  (tcols : pos { tcols /? cols })
+  (#f : perm)
+  requires
+    forall+
+      (tr : natlt (rows / trows))
+      (tc : natlt (cols / tcols)).
+        (exists* (em : ematrix et trows tcols).
+          gpu_matrix_subtile gm trows tcols tr tc |-> Frac f em)
+  ensures
+    (exists* (em : ematrix et rows cols). gm |-> Frac f em)
+{
+  admit();
+}
+
+ghost
+fn gpu_slice_gather_underspec
+  (#uid : int) (#a : Type u#0)
+  (#sz : nat)
+  (arr : gpu_array a sz)
+  (#f : perm)
+  (m n : nat)
+  (k : nat { k > 0 })
+  requires bigstar #uid 0 k (fun x -> exists* v. gpu_pts_to_slice arr #(f /. k) m n v)
+  ensures
+    exists* v.
+      gpu_pts_to_slice arr #f m n v
+{
+  // GUIDO: prove this later
+  admit();
+}
+
+ghost
+fn linearize_tile_indices
+  (#et : Type0)
+  (#rows #cols : nat)
+  (trows : nat{trows > 0 /\ trows /? rows})
+  (tcols : nat{tcols > 0 /\ tcols /? cols})
+  (#l : mlayout rows cols)
+  (gm : gpu_matrix et l)
+  (#f : perm)
+  (#em : ematrix et rows cols)
+  (n : nat {n == rows/trows * (cols/tcols)})
+requires
+  forall+ (tr: natlt (rows/trows)) (tc: natlt (cols/tcols)).
+    gpu_matrix_subtile gm trows tcols tr tc |-> Frac f (ematrix_subtile em trows tcols tr tc)
+ensures
+  forall+ (trc : natlt n).
+    gpu_matrix_subtile gm trows tcols (trc/(cols/tcols)) (trc%(cols/tcols))
+      |-> Frac f (ematrix_subtile em trows tcols (trc/(cols/tcols)) (trc%(cols/tcols)))
+{
+  forevery_unfactor' (n) (rows/trows) (cols/tcols) _;
+}
+
+ghost
+fn create_warp_tiles_shared
+  (#et : Type0) {| scalar et |}
+  (#rows #cols : nat)
+  (#l : mlayout rows cols)
+  ([@@@mkey] gm : gpu_matrix et l)
+  (#f : perm)
+  (#em : ematrix et rows cols)
+  (trows : nat{trows > 0 /\ trows /? rows})
+  (tcols : nat{tcols > 0 /\ tcols /? cols})
+  (nthr : nat{nthr == rows/trows * (cols/tcols) * warp_size})
+requires
+  gm |-> Frac f em
+ensures
+  forall+ (trc : natlt nthr).
+    warp_tile gm trows tcols (trc/warp_size)
+      |-> Frac (f /. warp_size)
+    (ematrix_subtile em trows tcols
+      (warp_tile_idx_rows rows cols trows tcols (trc/warp_size))
+      (warp_tile_idx_cols rows cols trows tcols (trc/warp_size)))
+{
+  gpu_matrix_tile gm trows tcols;
+  linearize_tile_indices trows tcols gm (rows/trows * (cols/tcols));
+
+  ghost
+  fn share_within_warp (trc : natlt (rows/trows * (cols/tcols)))
+  requires
+    gpu_matrix_subtile gm trows tcols (trc/(cols/tcols)) (trc%(cols/tcols))
+      |-> Frac f (ematrix_subtile em trows tcols (trc/(cols/tcols)) (trc%(cols/tcols)))
+  ensures
+    forall+ (_lid: natlt warp_size).
+      gpu_matrix_subtile gm trows tcols (trc/(cols/tcols)) (trc%(cols/tcols))
+        |-> Frac (f /. warp_size) (ematrix_subtile em trows tcols (trc/(cols/tcols)) (trc%(cols/tcols)))
+  {
+    gpu_matrix_share_n _ warp_size; 
+  };
+  forevery_map _ _ share_within_warp;
+  forevery_unfactor' nthr (rows / trows * (cols / tcols)) 32 _;
+  ();
+}
+
+ghost
+fn gpu_matrix_share_threads
+  (#et : Type)
+  (#rows #cols : nat)
+  (#l : mlayout rows cols)
+  (gm : gpu_matrix et l)
+  (#f : perm)
+  (#em : ematrix et rows cols)
+  (nblk nthr : pos)
+requires
+  gm |-> Frac f em
+ensures
+  forall+ (bid : natlt nblk) (tid : natlt nthr). gm |-> Frac (f/.(nblk*nthr)) em
+{
+  gpu_matrix_share_n gm (nblk*nthr);
+  forevery_factor (nblk * nthr) nblk nthr _;
+}
+
+ghost
+fn setup
+  (#et_ab #et_c : Type0)
+  {| scalar et_ab, scalar et_c |}
+  (#rows #shared #cols : szp)
+  (#lA : mlayout rows shared)
+  (#lB : mlayout shared cols)
+  (#lC : mlayout rows cols)
+  {| clayout lA, clayout lB, clayout lC |}
+  (gA : gpu_matrix et_ab lA)
+  (eA : ematrix et_ab rows shared)
+  (gB : gpu_matrix et_ab lB)
+  (eB : ematrix et_ab shared cols)
+  (gC : gpu_matrix et_c lC)
+  (eC : ematrix et_c rows cols)
+  (bm bn bk
+   tm tn tk
+   wm wn : szp { constraints bm bn bk tm tn tk wm wn })
+  (#_ : squash (bm /? rows))
+  (#_ : squash (bn /? cols))
+  (#_ : squash (SZ.fits (bm * bk) /\ SZ.fits (bk * bn)))
+  (nblk : szp{SZ.v nblk == rows/bm * (cols/bn)})
+  (nthr : szp{SZ.v nthr == bm/(wm*tm) * (bn/(wn*tn)) * warp_size})
+  (fA fB : perm)
+  ()
+  norewrite
+  requires
+    gA |-> Frac fA eA **
+    gB |-> Frac fB eB **
+    gC |-> eC
+  ensures
+    (forall+ (bid : natlt nblk)
+             (tid : natlt nthr).
+      kpre1 gA eA gB eB gC bm bn bk tm tn tk wm wn fA fB nthr bid tid) **
+    emp (* frame *)
+{
+  gpu_matrix_share_threads gA nblk nthr;
+  gpu_matrix_share_threads gB nblk nthr;
+  
+  gpu_matrix_tile gC bm bn;
+  linearize_tile_indices bm bn gC nblk;
+
+  forevery_map
+    (fun (trc : natlt nblk) ->
+      (gpu_matrix_subtile gC (SZ.v bm) (SZ.v bn) (trc/(cols/bn)) (trc%(cols/bn))) 
+        // Explicit fraction required, otherwise tactic to resolve it fails?!?!
+        |-> Frac 1.0R
+      (ematrix_subtile eC bm bn (trc/(cols/bn)) (trc%(cols/bn))))
+    _
+    (fun trc ->
+      create_warp_tiles_shared
+        (block_tile gC (SZ.v bm) (SZ.v bn) trc)
+        // (gpu_matrix_subtile gC (SZ.v bm) (SZ.v bn) (trc/(cols/bn)) (trc%(cols/bn)))
+        (wm*tm)
+        (wn*tn)
+        nthr);
+     
+  forevery_zip_2 #(natlt nblk) #_ #(natlt nthr)
+    (fun bid -> fun tid -> gB |-> Frac (fB /. (nblk*nthr)) eB)
+    (fun bid -> fun tid ->
+      (warp_tile (block_tile gC (SZ.v bm) (SZ.v bn) bid) (wm*tm) (wn*tn) (tid/warp_size))
+        |-> Frac (1.0R /. warp_size)
+      (ematrix_subtile (ematrix_subtile eC bm bn (bid/(cols/bn)) (bid%(cols/bn)))
+        (wm*tm) (wn*tn)
+        (warp_tile_idx_rows (SZ.v bm) (SZ.v bn) (wm*tm) (wn*tn) (tid/warp_size))
+        (warp_tile_idx_cols (SZ.v bm) (SZ.v bn) (wm*tm) (wn*tn) (tid/warp_size))));
+
+  forevery_zip_2 #(natlt nblk) #_ #(natlt nthr)
+    (fun bid -> fun tid -> gA |-> Frac (fA /. (nblk*nthr)) eA)
+    _;
+
+  // is this necessary? :/
+  ghost
+  fn aux (bid : natlt nblk) (tid : natlt nthr)
+  requires
+    gA |-> Frac (fA /. (nblk*nthr)) eA ** gB |-> Frac (fB /. (nblk*nthr)) eB **
+    (warp_tile (block_tile gC (SZ.v bm) (SZ.v bn) bid) (wm*tm) (wn*tn) (tid/warp_size))
+      |-> Frac (1.0R /. warp_size)
+    (ematrix_subtile (ematrix_subtile eC bm bn (bid/(cols/bn)) (bid%(cols/bn)))
+      (wm*tm) (wn*tn)
+      (warp_tile_idx_rows (SZ.v bm) (SZ.v bn) (wm*tm) (wn*tn) (tid/warp_size))
+      (warp_tile_idx_cols (SZ.v bm) (SZ.v bn) (wm*tm) (wn*tn) (tid/warp_size)))
+  ensures
+    gA |-> Frac (fA /. ((rows/bm) * (cols/bn) * nthr)) eA **
+    gB |-> Frac (fB /. ((rows/bm) * (cols/bn) * nthr)) eB **
+    live_warp_tile gC bm bn tm tn wm wn bid (tid/warp_size)
+  {
+    fold live_warp_tile gC bm bn tm tn wm wn bid (tid/warp_size);
+  };
+  forevery_map_2 _ _ aux;
+  ()
+}
+
+ghost
+fn lemma_even_barrier_p_to_q
+  (#et : Type0) {| has_vec_cpy et |}
+  (#bm #bn #bk : szp)
+  (l1 : full_mlayout bm bk)
+  (l2 : full_mlayout bk bn)
+  (sar1 : gpu_array et (bm * bk))
+  (sar2 : gpu_array et (bk * bn))
+  (nthr : pos)
+  (#_ : squash (chunk et /?+ bn))
+  (#_ : squash (chunk et /?+ bk))
+  (#_ : squash (chunk et * nthr /?+ (bm * bk)))
+  (#_ : squash (chunk et * nthr /?+ (bk * bn)))
+requires
+  forall+ (tid : natlt nthr).
+    (exists* (x : ematrix _ _ _). (from_array l1 sar1) |-> Frac (1.0R /. nthr) x) **
+    (exists* (x : ematrix _ _ _). (from_array l2 sar2) |-> Frac (1.0R /. nthr) x)
+ensures
+  forall+ (tid : natlt nthr).
+    live_tile_stride_cells (from_array l1 sar1) nthr tid **
+    live_tile_stride_cells (from_array l2 sar2) nthr tid
+{
+  admit();
+  // gpu_matrix_gather_n_underspec #_ #0 _ _;
+  with em. assert (from_array l1 sar1) |-> em;
+  gpu_matrix_explode _;
+  forevery_unfactor' (bm*bk) bm bk _;
+  assert pure (chunk et * nthr /?+ (bm * bk));
+  // FIXME the following assert fails
+  // assert pure (chunk et /?+ (bm * bk));
+  // assert pure (bm * bk / (chunk et) * (chunk et) == bm * bk);
+  admit();
+  forevery_iso_back #_ #_ #(natlt (bm*bk)) (bij_nat_prod #(bm*bk/(chunk et)) #(chunk et))
+    (fun (xy: natlt (bm*bk/(chunk et)) & natlt (chunk et)) ->
+      gpu_matrix_pts_to_cell (from_array l1 sar1)
+        ((xy._1 * (chunk et) + xy._2) / bk)
+        ((xy._1 * (chunk et) + xy._2) % bk)
+        (macc em ((xy._1 * (chunk et) + xy._2) / bk) ((xy._1 * (chunk et) + xy._2) % bk)));
+  admit();
+//
+//  forevery_unflatten (fun i -> fun j ->
+//    gpu_matrix_pts_to_cell (from_array l1 sar1)
+//        (xy / v bk)
+//        (xy % v bk)
+//        (macc em (xy / v bk) (xy % v bk)))
+//  forall+ (it : natlt (divup (rows*cols) (chunk et * nthr))).
+//    if (tid * + it * nthr) * chunk et / cols < rows
+//       && (tid * + it * nthr) * chunk et) % cols < cols - chunk et + 1
+//    then
+//       live_chunk (from_array l1 sar1)
+//         ((tid * + it * nthr) * chunk et / cols)
+//         ((tid * + it * nthr) * chunk et) % cols)
+//    else emp
+}
+
+ghost
+fn lemma_odd_barrier_p_to_q
+  (#et : Type0) {| has_vec_cpy et |}
+  (#bm #bn #bk : szp)
+  (l1 : full_mlayout bm bk)
+  (l2 : full_mlayout bk bn)
+  (sar1 : gpu_array et (bm * bk))
+  (sar2 : gpu_array et (bk * bn))
+  (nthr : pos)
+  (#_ : squash (chunk et /?+ bn))
+  (#_ : squash (chunk et /?+ bk))
+  (#_ : squash (chunk et * nthr /?+ (bm * bk)))
+  (#_ : squash (chunk et * nthr /?+ (bk * bn)))
+requires
+  forall+ (tid : natlt nthr).
+    live_tile_stride_cells (from_array l1 sar1) nthr tid **
+    live_tile_stride_cells (from_array l2 sar2) nthr tid
+ensures
+  forall+ (tid : natlt nthr).
+    (exists* (x : ematrix _ _ _). (from_array l1 sar1) |-> Frac (1.0R /. nthr) x) **
+    (exists* (x : ematrix _ _ _). (from_array l2 sar2) |-> Frac (1.0R /. nthr) x)
+{
+  (* analogous, but fill it in. *)
+  admit();
+}
+
+ghost
+fn barrier_p_to_q_transform
+  (#et : Type0) {| has_vec_cpy et |}
+  (#bm #bn #bk : szp)
+  (l1 : full_mlayout bm bk)
+  (l2 : full_mlayout bk bn)
+  (sar1 : gpu_array et (bm * bk))
+  (sar2 : gpu_array et (bk * bn))
+  (nthr : pos)
+  (#_ : squash (chunk et /?+ bn))
+  (#_ : squash (chunk et /?+ bk))
+  (#_ : squash (chunk et * nthr /?+ (bm * bk)))
+  (#_ : squash (chunk et * nthr /?+ (bk * bn)))
+  (it : nat)
+requires 
+  forall+ (tid : natlt nthr). barrier_p (from_array l1 sar1) (from_array l2 sar2) nthr it tid
+ensures
+  forall+ (tid : natlt nthr). barrier_q (from_array l1 sar1) (from_array l2 sar2) nthr it tid
+{
+  // requires ANF?
+  let ev = even it;
+  if ev {
+    ghost
+    fn evaux (tid : natlt nthr)
+      norewrite
+      requires
+        (barrier_p (from_array l1 sar1) (from_array l2 sar2) nthr) it tid
+      ensures
+        (exists* (x : ematrix _ _ _). (from_array l1 sar1) |-> Frac (1.0R /. nthr) x) **
+        (exists* (x : ematrix _ _ _). (from_array l2 sar2) |-> Frac (1.0R /. nthr) x)
+    {
+      rewrite barrier_p (from_array l1 sar1) (from_array l2 sar2) nthr it tid
+           as (exists* (x : ematrix _ _ _). (from_array l1 sar1) |-> Frac (1.0R /. nthr) x) **
+              (exists* (x : ematrix _ _ _). (from_array l2 sar2) |-> Frac (1.0R /. nthr) x);
+    };
+    forevery_map _ _ evaux;
+
+    lemma_even_barrier_p_to_q l1 l2 sar1 sar2 nthr;
+
+    ghost
+    fn evaux2 (tid : natlt nthr)
+    requires
+      live_tile_stride_cells (from_array l1 sar1) nthr tid **
+      live_tile_stride_cells (from_array l2 sar2) nthr tid
+    ensures
+      barrier_q (from_array l1 sar1) (from_array l2 sar2) nthr it tid
+    {
+      rewrite live_tile_stride_cells (from_array l1 sar1) nthr tid **
+              live_tile_stride_cells (from_array l2 sar2) nthr tid
+           as barrier_q (from_array l1 sar1) (from_array l2 sar2) nthr it tid;
+    };
+    forevery_map _ _ evaux2;
+  } else {
+    ghost
+    fn oddaux (tid : natlt nthr)
+      norewrite
+      requires
+        barrier_p (from_array l1 sar1) (from_array l2 sar2) nthr it tid
+      ensures
+        live_tile_stride_cells (from_array l1 sar1) nthr tid **
+        live_tile_stride_cells (from_array l2 sar2) nthr tid
+    {
+      rewrite barrier_p (from_array l1 sar1) (from_array l2 sar2) nthr it tid
+           as live_tile_stride_cells (from_array l1 sar1) nthr tid **
+              live_tile_stride_cells (from_array l2 sar2) nthr tid;
+    };
+
+    forevery_map _ _ oddaux;
+    lemma_odd_barrier_p_to_q l1 l2 sar1 sar2 nthr;
+
+    ghost
+    fn oddaux2 (tid : natlt nthr)
+      norewrite
+      requires
+        // explicit sizes are not helping
+        (exists* (x : ematrix et bm bk). (from_array l1 sar1) |-> Frac (1.0R /. nthr) x) **
+        (exists* (x : ematrix et bk bn). (from_array l2 sar2) |-> Frac (1.0R /. nthr) x)
+      ensures
+        barrier_q (from_array l1 sar1) (from_array l2 sar2) nthr it tid
+    {
+      // extra rewrite step reduces time for type checking by ~50%
+      rewrite 
+          (exists* (x : ematrix _ _ _). (from_array l1 sar1) |-> Frac (1.0R /. nthr) x) **
+          (exists* (x : ematrix _ _ _). (from_array l2 sar2) |-> Frac (1.0R /. nthr) x)
+      as 
+        (if even (it+1) then
+          (exists* (x : ematrix _ _ _). (from_array l1 sar1) |-> Frac (1.0R /. nthr) x) **
+          (exists* (x : ematrix _ _ _). (from_array l2 sar2) |-> Frac (1.0R /. nthr) x)
+        else
+          live_tile_stride_cells (from_array l1 sar1) nthr tid **
+          live_tile_stride_cells (from_array l2 sar2) nthr tid);
+      rewrite 
+        (if even (it+1) then
+          (exists* (x : ematrix _ _ _). (from_array l1 sar1) |-> Frac (1.0R /. nthr) x) **
+          (exists* (x : ematrix _ _ _). (from_array l2 sar2) |-> Frac (1.0R /. nthr) x)
+        else
+          live_tile_stride_cells (from_array l1 sar1) nthr tid **
+          live_tile_stride_cells (from_array l2 sar2) nthr tid)
+      as
+        barrier_q (from_array l1 sar1) (from_array l2 sar2) nthr it tid;
+    };
+    forevery_map _ _ oddaux2;
+  }
+}
+
+#set-options "--print_implicits"
+
+let frozen p = p
+
+ghost
+fn freeze (p : slprop)
+  requires p
+  ensures  frozen p
+{
+  rewrite p as frozen p;
+}
+
+ghost
+fn thaw (p : slprop)
+  requires frozen p
+  ensures  p
+{
+  rewrite frozen p as p;
+}
+
+ghost
+fn block_setup
+  (#et_ab #et_c : Type0)
+  {| scalar et_ab, has_vec_cpy et_ab, scalar et_c |}
+  (#rows #shared #cols : szp)
+  (#lA : mlayout rows shared)
+  (#lB : mlayout shared cols)
+  (#lC : mlayout rows cols)
+  {| clayout lA, clayout lB, clayout lC |}
+  (gA : gpu_matrix et_ab lA)
+  (eA : ematrix et_ab rows shared)
+  (gB : gpu_matrix et_ab lB)
+  (eB : ematrix et_ab shared cols)
+  (gC : gpu_matrix et_c lC)
+  (eC : ematrix et_c rows cols)
+  (bm bn bk
+   tm tn tk
+   wm wn : szp { constraints bm bn bk tm tn tk wm wn })
+  (#_ : squash (bm /?+ rows))
+  (#_ : squash (bn /?+ cols))
+  (#_ : squash (SZ.fits (bm * bk) /\ SZ.fits (bk * bn)))
+  (nblk : szp{SZ.v nblk == rows/bm * (cols/bn)})
+  (nthr : szp{SZ.v nthr == bm/(wm*tm) * (bn/(wn*tn)) * warp_size /\ nthr <= 1024})
+  (#_ : squash (chunk et_ab /?+ bn))
+  (#_ : squash (chunk et_ab /?+ bk))
+  (#_ : squash (chunk et_ab * nthr /?+ (bm * bk)))
+  (#_ : squash (chunk et_ab * nthr /?+ (bk * bn)))
+  (fA fB : perm)
+  (sh : c_shmems (shmems_desc et_ab bm bn bk))
+  (bid : natlt nblk)
+  ()
+  norewrite
+  requires
+    block_setup_tok nthr **
+    live_c_shmems sh **
+    (forall+ (tid : natlt nthr).
+      kpre1 gA eA gB eB gC bm bn bk tm tn tk wm wn fA fB nthr bid tid)
+  ensures
+    block_setup_tok nthr **
+    (forall+ (tid : natlt nthr).
+      kpre gA eA gB eB gC bm bn bk tm tn tk wm wn fA fB nthr sh bid tid) **
+    emp (* frame *)
+{
+  (* permissions for shared memory *)
+  // shmem for A tile
+  // rewrite each shmems_desc et_ab bm bn bk as [SHArray et_ab (bm *^ bk); SHArray et_ab (bk *^ bn);];
+  rewrite live_c_shmems sh as
+    live_c_shmem (fst sh) **
+    (live_c_shmem (fst (snd sh)) **
+     emp);
+  rewrite live_c_shmem (fst sh) as (exists* v. gpu_pts_to_array (fst sh) v);
+  rewrite live_c_shmem (fst (snd sh)) as (exists* v. gpu_pts_to_array (fst (snd sh)) v);
+  gpu_slice_share (fst sh) 0 (bm*bk) nthr;
+  gpu_slice_share (fst (snd sh)) 0 (bk*bn) nthr;
+  with s1.
+    assert (forall+ (x: natlt nthr). gpu_pts_to_slice (fst sh) #(1.0R /. nthr) 0 (bm*bk) (reveal s1));
+  with s2.
+    assert (forall+ (x: natlt nthr). gpu_pts_to_slice (fst (snd sh)) #(1.0R /. nthr) 0 (bk*bn) s2);
+
+  // introduce exists under forall+
+  // :( I do not see another way for introducing the exists
+  // gpu_pts_to_array (although unfold) does not work because the array sizes are not matched:
+  //  there are bm*^bk and bm*bk in the context. while gpu_pts_to_array uses either bm*^bk or bm*bk
+  // with s. assert (forall+ (x: natlt nthr). gpu_pts_to_array #_ #(bm*^bk) (fst sh) #(1.0R /. nthr) s);
+  ghost fn aux (#n : nat) (arr : gpu_array et_ab n) (s : erased (seq et_ab)) (tid : natlt nthr)
+    requires gpu_pts_to_slice arr #(1.0R /. nthr) 0 n s
+    ensures exists* (x : seq et_ab). gpu_pts_to_array arr #(1.0R /. nthr) x
+    {};
+  forevery_map #(natlt nthr)
+    (fun _tid -> gpu_pts_to_slice (fst sh) #(1.0R /. nthr) 0 (bm*bk) s1)
+    _ (aux (fst sh) s1);
+  forevery_map #(natlt nthr)
+    (fun _tid -> gpu_pts_to_slice (fst (snd sh)) #(1.0R /. nthr) 0 (bk*bn) s2)
+    _ (aux (fst (snd sh)) s2);
+
+  (* create barrier token *)
+  B.mk_barrier nthr _ _
+    (barrier_p_to_q_transform (R.row_major bm bk) (R.row_major bk bn) (fst sh) (fst (snd sh)) nthr);
+  let sar1 = fst sh;
+  let sar2 = fst (snd sh);
+
+  (* consolidate permissions under a single forall+ *)
+  forevery_zip
+    (fun tid -> exists* (x : seq et_ab). gpu_pts_to_array (fst (snd sh)) #(1.0R /. nthr) x)
+    (fun tid ->
+      barrier_tok (R.row_major bm bk) (R.row_major bk bn) (fst sh) (fst (snd sh)) 0 nthr tid)
+    ;
+  forevery_zip
+    (fun tid -> exists* (x : seq et_ab). gpu_pts_to_array (fst sh) #(1.0R /. nthr) x)
+    (fun tid ->
+      (exists* (x : seq et_ab). gpu_pts_to_array (fst (snd sh)) #(1.0R /. nthr) x) **
+      barrier_tok (R.row_major bm bk) (R.row_major bk bn) (fst sh) (fst (snd sh)) 0 nthr tid);
+  forevery_zip #(natlt nthr)
+    (fun tid -> kpre1 gA eA gB eB gC bm bn bk tm tn tk wm wn fA fB nthr bid tid) _;
+  ()
+}
+
+ghost
+fn block_teardown
+  (#et_ab #et_c : Type0)
+  {| scalar et_ab, has_vec_cpy et_ab, scalar et_c |}
+  (#rows #shared #cols : szp)
+  (#lA : mlayout rows shared)
+  (#lB : mlayout shared cols)
+  (#lC : mlayout rows cols)
+  (gA : gpu_matrix et_ab lA)
+  (eA : ematrix et_ab rows shared)
+  (gB : gpu_matrix et_ab lB)
+  (eB : ematrix et_ab shared cols)
+  (gC : gpu_matrix et_c lC)
+  (eC : ematrix et_c rows cols)
+  (bm bn bk
+   tm tn tk
+   wm wn : szp { constraints bm bn bk tm tn tk wm wn })
+  (#_ : squash (bm /?+ rows))
+  (#_ : squash (bn /?+ cols))
+  (#_ : squash (SZ.fits (bm * bk) /\ SZ.fits (bk * bn)))
+  (nblk : szp{SZ.v nblk == rows/bm * (cols/bn)})
+  (nthr : szp{SZ.v nthr == bm/(wm*tm) * (bn/(wn*tn)) * warp_size})
+  (fA fB : perm)
+  (sh : c_shmems (shmems_desc et_ab bm bn bk))
+  (bid : natlt nblk)
+  ()
+  norewrite
+  requires
+    (forall+ (tid : natlt nthr).
+      kpost (* comb *) gA eA gB eB gC bm bn bk tm tn tk wm wn fA fB nthr sh bid tid) **
+    emp (* frame *)
+  ensures
+    live_c_shmems sh **
+    (forall+ (tid : natlt nthr).
+      kpost1 (* comb *) gA eA gB eB gC bm bn bk tm tn tk wm wn fA fB nthr bid tid)
+{
+  forevery_unzip #(natlt nthr)
+    (fun tid -> kpost1 gA eA gB eB gC bm bn bk tm tn tk wm wn fA fB nthr bid tid)
+    _;
+  forevery_unzip #(natlt nthr)
+    (fun _tid -> ((exists* (x: seq et_ab). gpu_pts_to_array (fst sh) #(1.0R /. nthr) x)))
+    _;
+  forevery_unzip #(natlt nthr)
+    (fun _tid -> ((exists* (x: seq et_ab). gpu_pts_to_array (fst (snd sh)) #(1.0R /. nthr) x)))
+    _;
+  
+  forevery_tostar #(natlt nthr)
+    (fun _tid -> ((exists* (x: seq et_ab). gpu_pts_to_array (fst sh) #(1.0R /. nthr) x)));
+  forevery_tostar #(natlt nthr)
+    (fun _tid -> ((exists* (x: seq et_ab). gpu_pts_to_array (fst (snd sh)) #(1.0R /. nthr) x)));
+  
+  // rewrite each Kuiper.Enumerable.cardinal (natlt nthr) #_ as SZ.v nthr;
+  gpu_slice_gather_underspec (fst sh) 0 (bm*^bk) nthr;
+  gpu_slice_gather_underspec (fst (snd sh)) 0 (bk*^bn) nthr;
+
+  assert (exists* v. gpu_pts_to_array (fst sh) v);
+  rewrite (exists* v. gpu_pts_to_array (fst sh) v) as live_c_shmem (fst sh);
+  rewrite (exists* v. gpu_pts_to_array (fst (snd sh)) v) as live_c_shmem (fst (snd sh));
+  rewrite
+    live_c_shmem (fst sh) **
+    (live_c_shmem (fst (snd sh)) **
+     emp)
+    as 
+    live_c_shmems sh;
+
+  drop_
+    (forall+ (x: natlt nthr).
+      barrier_tok (R.row_major bm bk) (R.row_major bk bn) (fst sh) (fst (snd sh)) (2 * (shared/bk)) nthr x);
+  ()
+}
+
+ghost
+fn untile_warp_tiles_shared
+  (#et : Type0) {| scalar et |}
+  (#rows #cols : nat)
+  (#l : mlayout rows cols)
+  ([@@@mkey] gm : gpu_matrix et l)
+  (#f : perm)
+  (trows : nat{trows > 0 /\ trows /? rows})
+  (tcols : nat{tcols > 0 /\ tcols /? cols})
+  (nthr : nat{nthr == rows/trows * (cols/tcols) * warp_size})
+requires
+  forall+ (tid : natlt nthr).
+    (exists* (em : ematrix _ _ _).
+      gpu_matrix_subtile gm trows tcols
+        (warp_tile_idx_rows rows cols trows tcols (tid/warp_size))
+        (warp_tile_idx_cols rows cols trows tcols (tid/warp_size))
+      |-> Frac (f /. warp_size) em)
+ensures
+  (exists* (em : ematrix _ _ _). gm |-> Frac f em)
+{
+  admit();
+  // forevery_iso #(natlt nthr) (bij_self (natlt (rows/trows * (cols/tcols) * warp_size))) _;
+  // forevery_unflatten_natlt 
+  //   (fun (trc : natlt (rows/trows * (cols/tcols))) -> fun (_lid : natlt warp_size) ->
+  //     (exists* (em : ematrix _ _ _).
+  //       gpu_matrix_subtile gm trows tcols
+  //         (warp_tile_idx_rows rows cols trows tcols (trc))
+  //         (warp_tile_idx_cols rows cols trows tcols (trc))
+  //     |-> Frac (f /. warp_size) em));
+
+  // ghost
+  // fn unshare_within_warp (wid : natlt (rows/trows * (cols/tcols)))
+  // requires
+  //   forall+ (_lid: natlt warp_size). (exists* (em : ematrix _ _ _).
+  //     gpu_matrix_subtile gm trows tcols (wid/(cols/tcols)) (wid%(cols/tcols))
+  //       |-> Frac (f /. warp_size) em)
+  // ensures
+  //   (exists* (em : ematrix _ _ _).
+  //     gpu_matrix_subtile gm trows tcols (wid/(cols/tcols)) (wid%(cols/tcols))
+  //       |-> Frac f em)
+  // {
+  //   forevery_tostar (fun (lid : natlt warp_size) ->
+  //    (exists* (em : ematrix _ _ _).
+  //       gpu_matrix_subtile gm trows tcols (wid/(cols/tcols)) (wid%(cols/tcols))
+  //         |-> Frac (f /. warp_size) em));
+  //   rewrite each Kuiper.Enumerable.cardinal (natlt warp_size) #_ as warp_size;
+  //   gpu_matrix_gather_n_underspec
+  //     (gpu_matrix_subtile gm trows tcols (wid/(cols/tcols)) (wid%(cols/tcols)))
+  //     warp_size;
+  // };
+  // forevery_map _ _ unshare_within_warp;
+  // forevery_unflatten_natlt 
+  //   (fun (trow : natlt (rows/trows)) -> fun (tcol : natlt (cols/tcols)) ->
+  //     (exists* (em : ematrix et trows tcols).
+  //       (gpu_matrix_subtile gm trows tcols trow tcol) |-> Frac f em));
+  // gpu_matrix_untile_underspec gm trows tcols;
+}
+
+ghost
+fn forevery_factor'
+  (n : nat)
+  (d1 : nat) (d2 : nat { n == d1 * d2 })
+  (p : natlt d1 -> natlt d2 -> slprop)
+  requires
+    forall+ (i:natlt n). p (i / d2) (i % d2)
+  ensures
+    forall+ (i1:natlt d1) (i2:natlt d2). p i1 i2
+{
+  forevery_factor n d1 d2 (fun i -> p (i / d2) (i % d2));
+  forevery_ext_2
+    (fun (i1 : natlt d1) (i2 : natlt d2) -> p ((i1 * d2 + i2) / d2) ((i1 * d2 + i2) % d2))
+    (fun (i1 : natlt d1) (i2 : natlt d2) -> p i1 i2);
+  ();
+}
+
+ghost
+fn teardown
+  (#et_ab #et_c : Type0)
+  {| scalar et_ab, has_vec_cpy et_ab, scalar et_c |}
+  (#rows #shared #cols : szp)
+  (#lA : mlayout rows shared)
+  (#lB : mlayout shared cols)
+  (#lC : mlayout rows cols)
+  (gA : gpu_matrix et_ab lA)
+  (eA : ematrix et_ab rows shared)
+  (gB : gpu_matrix et_ab lB)
+  (eB : ematrix et_ab shared cols)
+  (gC : gpu_matrix et_c lC)
+  (eC : ematrix et_c rows cols)
+  (bm bn bk
+   tm tn tk
+   wm wn : szp { constraints bm bn bk tm tn tk wm wn })
+  (#_ : squash (bm /?+ rows))
+  (#_ : squash (bn /?+ cols))
+  (#_ : squash (SZ.fits (bm * bk) /\ SZ.fits (bk * bn)))
+  (nblk : szp{SZ.v nblk == rows/bm * (cols/bn)})
+  (nthr : szp{SZ.v nthr == bm/(wm*tm) * (bn/(wn*tn)) * warp_size})
+  (#_ : squash (chunk et_ab * nthr /?+ (bm * bk)))
+  (#_ : squash (chunk et_ab * nthr /?+ (bk * bn)))
+  (fA fB : perm)
+  ()
+  norewrite
+  requires
+    (forall+ (bid : natlt nblk)
+             (tid : natlt nthr).
+      kpost1 gA eA gB eB gC bm bn bk tm tn tk wm wn fA fB nthr bid tid) **
+    emp
+  ensures
+    gA |-> Frac fA eA **
+    gB |-> Frac fB eB **
+    // underspec not implemented anyway
+    (exists* eC'. gC |-> eC')
+{
+  forevery_unfactor' (rows/bm * (cols/bn) * nthr) nblk nthr _;
+  forevery_unzip _ _; 
+  forevery_unzip _ _; 
+
+  gpu_matrix_gather_n gA (rows/bm * (cols/bn) * nthr);
+  gpu_matrix_gather_n gB (rows/bm * (cols/bn) * nthr);
+
+  forevery_factor'
+    (rows/bm * (cols/bn) * nthr)
+    (rows/bm * (cols/bn))
+    nthr
+    (fun (bid : natlt (rows/bm * (cols/bn))) (tid : natlt nthr) ->
+      live_warp_tile #et_c #_ #(hide #nat (v rows)) #(v cols) #lC gC (v bm)
+            (v bn) (v tm) (v tn) (v wm) (v wn)
+            bid (tid / 32));
+
+  ghost
+  fn aux (bid : natlt nblk) (tid : natlt nthr)
+  requires live_warp_tile gC bm bn tm tn wm wn (bid) (tid/warp_size)
+  ensures live (
+        gpu_matrix_subtile
+          (gpu_matrix_subtile gC (SZ.v bm) (SZ.v bn)
+            (block_tile_idx_rows (SZ.v rows) (SZ.v cols) (SZ.v bm) (SZ.v bn) bid)
+            (block_tile_idx_cols (SZ.v rows) (SZ.v cols) (SZ.v bm) (SZ.v bn) bid))
+          (wm*tm) (wn*tn)
+          (warp_tile_idx_rows (SZ.v bm) (SZ.v bn) (wm*tm) (wn*tn) (tid/warp_size))
+          (warp_tile_idx_cols (SZ.v bm) (SZ.v bn) (wm*tm) (wn*tn) (tid/warp_size)))
+        #(1.0R /. warp_size)
+  {
+    rewrite live_warp_tile gC bm bn tm tn wm wn (bid) (tid/warp_size)
+    as
+      live (
+        gpu_matrix_subtile
+          (gpu_matrix_subtile gC (SZ.v bm) (SZ.v bn)
+            (block_tile_idx_rows (SZ.v rows) (SZ.v cols) (SZ.v bm) (SZ.v bn) bid)
+            (block_tile_idx_cols (SZ.v rows) (SZ.v cols) (SZ.v bm) (SZ.v bn) bid))
+          (wm*tm) (wn*tn)
+          (warp_tile_idx_rows (SZ.v bm) (SZ.v bn) (wm*tm) (wn*tn) (tid/warp_size))
+          (warp_tile_idx_cols (SZ.v bm) (SZ.v bn) (wm*tm) (wn*tn) (tid/warp_size)))
+        #(1.0R /. warp_size);
+  };
+  forevery_map_2 #(natlt (rows/bm * (cols/bn))) #(natlt nthr) _ _ aux;
+
+  forevery_map
+    (fun (bid : natlt ((rows/bm * (cols/bn)))) -> forall+ (tid: natlt nthr).
+      exists* (em: ematrix et_c (wm * tm) (wn * tn)).
+        gpu_matrix_subtile
+          (gpu_matrix_subtile gC (v bm) (v bn) (bid / (cols/bn)) (bid % (cols/bn)))
+              (wm*tm)
+              (wn*tn)
+              (tid / 32 / (bn / (wn*tn)))
+              (tid / 32 % (bn / (wn*tn))) |-> Frac (1.0R /. warp_size) em)
+    _
+    (fun (bid : natlt nblk) -> (untile_warp_tiles_shared
+        (gpu_matrix_subtile gC (SZ.v bm) (SZ.v bn)
+          (block_tile_idx_rows (SZ.v rows) (SZ.v cols) (SZ.v bm) (SZ.v bn) bid)
+          (block_tile_idx_cols (SZ.v rows) (SZ.v cols) (SZ.v bm) (SZ.v bn) bid))
+        (wm*tm) (wn*tn) nthr));
+
+  forevery_factor' ((rows/bm) * (cols/bn)) (rows/bm) (cols/bn)
+    (fun (trow : natlt (rows/bm)) -> fun (tcol : natlt (cols/bn)) ->
+      (exists* (em : ematrix et_c bm bn).
+        (gpu_matrix_subtile gC (SZ.v bm) (SZ.v bn) trow tcol) |-> em));
+  gpu_matrix_untile_underspec gC bm bn;
+  ()
+}
