src/lib/poly/gemm/Kuiper.Poly.GEMM.TensorCore2D.KernelDesc.fsti
@@ -1,0 +1,401 @@
+module Kuiper.Poly.GEMM.TensorCore2D.KernelDesc
+
+#lang-pulse
+
+#set-options "--z3rlimit 40"
+
+open Kuiper
+
+open Kuiper.Matrix.Reprs
+module R = Kuiper.Matrix.Reprs
+open Kuiper.TensorCore
+
+module SZ = Kuiper.SizeT
+open Kuiper.Matrix.Reprs.Type
+open Kuiper.Math { even, odd, even_2x, odd_2x1 }
+
+open Kuiper.Array.Vectorized { has_vec_cpy, chunk }
+open Kuiper.Matrix
+
+module MS = Kuiper.Spec.GEMM
+module SZ = Kuiper.SizeT
+module B = Kuiper.Barrier
+
+open Kuiper.Matrix.Reprs
+module R = Kuiper.Matrix.Reprs
+
+open Kuiper.EMatrix
+open Kuiper.VArray {
+  varray,
+  varray_pts_to,
+  varray_pts_to_cell
+}
+open Kuiper.TensorCore
+open Kuiper.Float16
+open Kuiper.Matrix.Tiling
+
+open Kuiper.Poly.GEMM.Copy.Vec
+open Kuiper.Poly.GEMM.Tiled.Common.Vec
+
+open Pulse.Lib.Array
+open Pulse.Lib.Trade
+
+open Kuiper.Bijection
+
+type constraints (bm bn bk tm tn tk wm wn : szp) : prop =
+  tm /?+ bm /\
+  tn /?+ bn /\
+  tk /?+ bk /\
+  wm * tm /?+ bm /\
+  wn * tn /?+ bn /\
+  SZ.fits (wm * wn)
+
+let live_warp_tile
+  (#et : Type0) {| scalar et |}
+  // Since this is an slprop, I would like to not erase the nat.
+  // Unfortunately, when unfolding live_warp_tile, after passing
+  // a (reveal x) as argument, this leads to (reveal (hide (reveal x)))
+  // which creates problems with type equalities.
+  (#rows : erased nat)
+  (#cols : nat)
+  (#lC : mlayout rows cols)
+  (gC : gpu_matrix et lC)
+  (bm : pos{bm /?+ rows})
+  (bn : pos{bn /?+ cols})
+  (tm : pos{tm /?+ bm})
+  (tn : pos{tn /?+ bn})
+  (wm : pos{wm * tm /?+ bm})
+  (wn : pos{wn * tn /?+ bn})
+  (bid : natlt ((rows/bm) * (cols/bn)))
+  (wid : natlt (bm/(wm*tm) * (bn/(wn*tn))))
+  : slprop
+  =
+  live (warp_tile (block_tile gC bm bn bid) (wm*tm) (wn*tn) wid) #(1.0R /. warp_size)
+
+let barrier_p
+  (#et : Type0) {| has_vec_cpy et |}
+  (#bm #bn #bk : szp)
+  (#l1 : mlayout bm bk)
+  (#l2 : mlayout bk bn)
+  (m1 : gpu_matrix et l1)
+  (m2 : gpu_matrix et l2)
+  (nthr : pos)
+  : B.barrier_side nthr =
+  fun it tid ->
+    if even it then
+      (exists* (x : ematrix _ _ _). m1 |-> Frac (1.0R /. nthr) x) **
+      (exists* (x : ematrix _ _ _). m2 |-> Frac (1.0R /. nthr) x)
+    else
+      live_tile_stride_cells m1 nthr tid **
+      live_tile_stride_cells m2 nthr tid
+
+let barrier_q
+  (#et : Type0) {| has_vec_cpy et |}
+  (#bm #bn #bk : szp)
+  (#l1 : mlayout bm bk)
+  (#l2 : mlayout bk bn)
+  (m1 : gpu_matrix et l1)
+  (m2 : gpu_matrix et l2)
+  (nthr : pos)
+  : B.barrier_side nthr =
+  fun it tid -> barrier_p m1 m2 nthr (it+1) tid (* flip flop *)
+
+let barrier_tok
+  (#et : Type0) {| has_vec_cpy et |}
+  (#bm #bn #bk : szp)
+  (* This is defined over the base shared gpu_arrays, as
+  this spec must make sense before the arrays are viewed as
+  a matrix. *)
+  (l1 : full_mlayout bm bk)
+  (l2 : full_mlayout bk bn)
+  (sar1 : gpu_array et (bm * bk))
+  (sar2 : gpu_array et (bk * bn))
+  (it : nat)
+  (nthr : pos)
+  (tid : natlt nthr)
+  : slprop
+  =
+  B.barrier_tok (barrier_p (from_array l1 sar1) (from_array l2 sar2) nthr)
+                (barrier_q (from_array l1 sar1) (from_array l2 sar2) nthr)
+                it tid
+
+unfold
+let kpre1
+  (#et_ab #et_c : Type0) {| scalar et_ab, scalar et_c |}
+  (#rows #shared #cols : szp)
+  (#lA : mlayout rows shared)
+  (#lB : mlayout shared cols)
+  (#lC : mlayout rows cols)
+  (gA : gpu_matrix et_ab lA)
+  (eA : ematrix et_ab rows shared)
+  (gB : gpu_matrix et_ab lB)
+  (eB : ematrix et_ab shared cols)
+  (gC : gpu_matrix et_c lC)
+  (bm bn bk
+   tm tn tk
+   wm wn : szp { constraints bm bn bk tm tn tk wm wn })
+  (#_ : squash (bm /?+ rows))
+  (#_ : squash (bn /?+ cols))
+  (fA fB : perm)
+  (nthr : nat {nthr == bm/(wm*tm)*(bn/(wn*tn))*warp_size})
+  (bid : enatlt (rows/bm * (cols/bn)))
+  (tid : enatlt nthr)
+  : slprop
+  =
+  gA |-> Frac (fA /. (rows/bm * (cols/bn) * nthr)) eA **
+  gB |-> Frac (fB /. (rows/bm * (cols/bn) * nthr)) eB **
+  live_warp_tile gC bm bn tm tn wm wn bid (tid/warp_size)
+  
+ghost
+fn simplif_rewrite_helper (#n1 #n2 : nat) (p : (natlt n1 & natlt n2) -> slprop) (trc: natlt (n1 * n2))
+  requires
+    (let g = (bij_nat_prod #n1 #n2).gg trc in p g)
+  ensures
+    p (Mktuple2 #(natlt n1) #(natlt n2) (trc / n2) (trc % n2))
+{
+  rewrite each (bij_nat_prod #n1 #n2).gg trc
+  as Mktuple2 #(natlt n1) #(natlt n2) (trc / n2) (trc % n2);
+}
+
+unfold
+let kpre
+  (#et_ab #et_c : Type0) {| scalar et_ab, has_vec_cpy et_ab, scalar et_c |}
+  (#rows #shared #cols : szp)
+  (#lA : mlayout rows shared)
+  (#lB : mlayout shared cols)
+  (#lC : mlayout rows cols)
+  (gA : gpu_matrix et_ab lA)
+  (eA : ematrix et_ab rows shared)
+  (gB : gpu_matrix et_ab lB)
+  (eB : ematrix et_ab shared cols)
+  (gC : gpu_matrix et_c lC)
+  (bm bn bk
+   tm tn tk
+   wm wn : szp { constraints bm bn bk tm tn tk wm wn })
+  (#_ : squash (bm /?+ rows))
+  (#_ : squash (bn /?+ cols))
+  (#_ : squash (SZ.fits (bm * bk) /\ SZ.fits (bk * bn)))
+  (fA fB : perm)
+  (nthr : nat {nthr == bm/(wm*tm)*(bn/(wn*tn))*warp_size})
+  (#_ : squash (1.0R /. nthr >=. 0.0R)) // to help SMT, this is obvious
+  (sh : c_shmems (shmems_desc et_ab bm bn bk))
+  (bid : natlt (rows/bm * (cols/bn)))
+  (tid : natlt nthr)
+  : slprop
+  =
+  kpre1 gA eA gB eB gC bm bn bk tm tn tk wm wn fA fB nthr bid tid **
+  (exists* (x : seq et_ab). gpu_pts_to_array (fst sh)       #(1.0R /. nthr) x) **
+  (exists* (x : seq et_ab). gpu_pts_to_array (fst (snd sh)) #(1.0R /. nthr) x) **
+  barrier_tok (R.row_major bm bk) (R.row_major bk bn) (fst sh) (fst (snd sh)) 0 nthr tid
+
+ghost
+fn setup
+  (#et_ab #et_c : Type0)
+  {| scalar et_ab, scalar et_c |}
+  (#rows #shared #cols : szp)
+  (#lA : mlayout rows shared)
+  (#lB : mlayout shared cols)
+  (#lC : mlayout rows cols)
+  {| clayout lA, clayout lB, clayout lC |}
+  (gA : gpu_matrix et_ab lA)
+  (eA : ematrix et_ab rows shared)
+  (gB : gpu_matrix et_ab lB)
+  (eB : ematrix et_ab shared cols)
+  (gC : gpu_matrix et_c lC)
+  (eC : ematrix et_c rows cols)
+  (bm bn bk
+   tm tn tk
+   wm wn : szp { constraints bm bn bk tm tn tk wm wn })
+  (#_ : squash (bm /? rows))
+  (#_ : squash (bn /? cols))
+  (#_ : squash (SZ.fits (bm * bk) /\ SZ.fits (bk * bn)))
+  (nblk : szp{SZ.v nblk == rows/bm * (cols/bn)})
+  (nthr : szp{SZ.v nthr == bm/(wm*tm) * (bn/(wn*tn)) * warp_size})
+  (fA fB : perm)
+  ()
+  norewrite
+  requires
+    gA |-> Frac fA eA **
+    gB |-> Frac fB eB **
+    gC |-> eC
+  ensures
+    (forall+ (bid : natlt nblk)
+             (tid : natlt nthr).
+      kpre1 gA eA gB eB gC bm bn bk tm tn tk wm wn fA fB nthr bid tid) **
+    emp (* frame *)
+
+ghost
+fn block_setup
+  (#et_ab #et_c : Type0)
+  {| scalar et_ab, has_vec_cpy et_ab, scalar et_c |}
+  (#rows #shared #cols : szp)
+  (#lA : mlayout rows shared)
+  (#lB : mlayout shared cols)
+  (#lC : mlayout rows cols)
+  {| clayout lA, clayout lB, clayout lC |}
+  (gA : gpu_matrix et_ab lA)
+  (eA : ematrix et_ab rows shared)
+  (gB : gpu_matrix et_ab lB)
+  (eB : ematrix et_ab shared cols)
+  (gC : gpu_matrix et_c lC)
+  (eC : ematrix et_c rows cols)
+  (bm bn bk
+   tm tn tk
+   wm wn : szp { constraints bm bn bk tm tn tk wm wn })
+  (#_ : squash (bm /?+ rows))
+  (#_ : squash (bn /?+ cols))
+  (#_ : squash (SZ.fits (bm * bk) /\ SZ.fits (bk * bn)))
+  (nblk : szp{SZ.v nblk == rows/bm * (cols/bn)})
+  (nthr : szp{SZ.v nthr == bm/(wm*tm) * (bn/(wn*tn)) * warp_size /\ nthr <= 1024})
+  (#_ : squash (chunk et_ab /?+ bn))
+  (#_ : squash (chunk et_ab /?+ bk))
+  (#_ : squash (chunk et_ab * nthr /?+ (bm * bk)))
+  (#_ : squash (chunk et_ab * nthr /?+ (bk * bn)))
+  (fA fB : perm)
+  (sh : c_shmems (shmems_desc et_ab bm bn bk))
+  (bid : natlt nblk)
+  ()
+  norewrite
+  requires
+    block_setup_tok nthr **
+    live_c_shmems sh **
+    (forall+ (tid : natlt nthr).
+      kpre1 gA eA gB eB gC bm bn bk tm tn tk wm wn fA fB nthr bid tid)
+  ensures
+    block_setup_tok nthr **
+    (forall+ (tid : natlt nthr).
+      kpre gA eA gB eB gC bm bn bk tm tn tk wm wn fA fB nthr sh bid tid) **
+    emp (* frame *)
+
+unfold
+let kpost1
+  (#et_ab #et_c : Type0) {| scalar et_ab, scalar et_c |}
+  (#rows #shared #cols : szp)
+  (#lA : mlayout rows shared)
+  (#lB : mlayout shared cols)
+  (#lC : mlayout rows cols)
+  (gA : gpu_matrix et_ab lA)
+  (eA : ematrix et_ab rows shared)
+  (gB : gpu_matrix et_ab lB)
+  (eB : ematrix et_ab shared cols)
+  (gC : gpu_matrix et_c lC)
+  (bm bn bk
+   tm tn tk
+   wm wn : szp { constraints bm bn bk tm tn tk wm wn })
+  (#_ : squash (bm /?+ rows))
+  (#_ : squash (bn /?+ cols))
+  (fA fB : perm)
+  (nthr : nat {nthr == bm/(wm*tm)*(bn/(wn*tn))*warp_size})
+  (bid : enatlt (rows/bm * (cols/bn)))
+  (tid : enatlt nthr)
+  : slprop
+  =
+  gA |-> Frac (fA /. (rows/bm * (cols/bn) * nthr)) eA **
+  gB |-> Frac (fB /. (rows/bm * (cols/bn) * nthr)) eB **
+  live_warp_tile gC bm bn tm tn wm wn bid (tid/warp_size)
+
+unfold
+let kpost
+  (#et_ab #et_c : Type0) {| scalar et_ab, has_vec_cpy et_ab, scalar et_c |}
+  (#rows #shared #cols : szp)
+  (#lA : mlayout rows shared)
+  (#lB : mlayout shared cols)
+  (#lC : mlayout rows cols)
+  (gA : gpu_matrix et_ab lA)
+  (eA : ematrix et_ab rows shared)
+  (gB : gpu_matrix et_ab lB)
+  (eB : ematrix et_ab shared cols)
+  (gC : gpu_matrix et_c lC)
+  (bm bn bk
+   tm tn tk
+   wm wn : szp { constraints bm bn bk tm tn tk wm wn
+                 /\ 2 * (shared / bk) >= 0 // obvious, but SMT is flaky
+                 })
+  (#_ : squash (bm /?+ rows))
+  (#_ : squash (bn /?+ cols))
+  (#_ : squash (SZ.fits (bm * bk) /\ SZ.fits (bk * bn)))
+  (fA fB : perm)
+  (nthr : nat {nthr == bm/(wm*tm)*(bn/(wn*tn))*warp_size})
+  (sh : c_shmems (shmems_desc et_ab bm bn bk))
+  (bid : natlt (rows/bm * (cols/bn)))
+  (tid : natlt nthr)
+  : slprop
+  =
+  kpost1 gA eA gB eB gC bm bn bk tm tn tk wm wn fA fB nthr bid tid **
+  (exists* (x : seq et_ab). (fst sh) |-> Frac (1.0R /. nthr) x) **
+  (exists* (x : seq et_ab). (fst (snd sh)) |-> Frac (1.0R /. nthr) x) **
+  barrier_tok (R.row_major bm bk) (R.row_major bk bn) (fst sh) (fst (snd sh)) (2 * (shared/bk)) nthr tid
+
+ghost
+fn block_teardown
+  (#et_ab #et_c : Type0)
+  {| scalar et_ab, has_vec_cpy et_ab, scalar et_c |}
+  (#rows #shared #cols : szp)
+  (#lA : mlayout rows shared)
+  (#lB : mlayout shared cols)
+  (#lC : mlayout rows cols)
+  (gA : gpu_matrix et_ab lA)
+  (eA : ematrix et_ab rows shared)
+  (gB : gpu_matrix et_ab lB)
+  (eB : ematrix et_ab shared cols)
+  (gC : gpu_matrix et_c lC)
+  (eC : ematrix et_c rows cols)
+  (bm bn bk
+   tm tn tk
+   wm wn : szp { constraints bm bn bk tm tn tk wm wn })
+  (#_ : squash (bm /?+ rows))
+  (#_ : squash (bn /?+ cols))
+  (#_ : squash (SZ.fits (bm * bk) /\ SZ.fits (bk * bn)))
+  (nblk : szp{SZ.v nblk == rows/bm * (cols/bn)})
+  (nthr : szp{SZ.v nthr == bm/(wm*tm) * (bn/(wn*tn)) * warp_size})
+  (fA fB : perm)
+  (sh : c_shmems (shmems_desc et_ab bm bn bk))
+  (bid : natlt nblk)
+  ()
+  norewrite
+  requires
+    (forall+ (tid : natlt nthr).
+      kpost (* comb *) gA eA gB eB gC bm bn bk tm tn tk wm wn fA fB nthr sh bid tid) **
+    emp (* frame *)
+  ensures
+    live_c_shmems sh **
+    (forall+ (tid : natlt nthr).
+      kpost1 (* comb *) gA eA gB eB gC bm bn bk tm tn tk wm wn fA fB nthr bid tid)
+
+ghost
+fn teardown
+  (#et_ab #et_c : Type0)
+  {| scalar et_ab, has_vec_cpy et_ab, scalar et_c |}
+  (#rows #shared #cols : szp)
+  (#lA : mlayout rows shared)
+  (#lB : mlayout shared cols)
+  (#lC : mlayout rows cols)
+  (gA : gpu_matrix et_ab lA)
+  (eA : ematrix et_ab rows shared)
+  (gB : gpu_matrix et_ab lB)
+  (eB : ematrix et_ab shared cols)
+  (gC : gpu_matrix et_c lC)
+  (eC : ematrix et_c rows cols)
+  (bm bn bk
+   tm tn tk
+   wm wn : szp { constraints bm bn bk tm tn tk wm wn })
+  (#_ : squash (bm /?+ rows))
+  (#_ : squash (bn /?+ cols))
+  (#_ : squash (SZ.fits (bm * bk) /\ SZ.fits (bk * bn)))
+  (nblk : szp{SZ.v nblk == rows/bm * (cols/bn)})
+  (nthr : szp{SZ.v nthr == bm/(wm*tm) * (bn/(wn*tn)) * warp_size})
+  (#_ : squash (chunk et_ab * nthr /?+ (bm * bk)))
+  (#_ : squash (chunk et_ab * nthr /?+ (bk * bn)))
+  (fA fB : perm)
+  ()
+  norewrite
+  requires
+    (forall+ (bid : natlt nblk)
+             (tid : natlt nthr).
+      kpost1 gA eA gB eB gC bm bn bk tm tn tk wm wn fA fB nthr bid tid) **
+    emp
+  ensures
+    gA |-> Frac fA eA **
+    gB |-> Frac fB eB **
+    // underspec not implemented anyway
+    (exists* eC'. gC |-> eC')
